---
title: "10-1 å€’ç«‹æŒ¯å­ãƒ¢ãƒ‡ãƒ«ï¼šéç·šå½¢ â†’ ç·šå½¢åŒ– â†’ çŠ¶æ…‹ç©ºé–“"
emoji: "ğŸ¯"
type: "tech"
topics: ["åˆ¶å¾¡", "å€’ç«‹æŒ¯å­", "çŠ¶æ…‹ç©ºé–“", "ç·šå½¢åŒ–"]
published: false
---

# 10-1 å€’ç«‹æŒ¯å­ãƒ¢ãƒ‡ãƒ«ï¼šéç·šå½¢ â†’ ç·šå½¢åŒ– â†’ çŠ¶æ…‹ç©ºé–“

---

## 1. ãƒ¢ãƒ‡ãƒ«å®šç¾©ï¼ˆcart-poleï¼‰

- å°è»Šè³ªé‡ï¼šM [kg]
- æŒ¯å­è³ªé‡ï¼šm [kg]
- æŒ¯å­é•·ï¼ˆæ”¯ç‚¹ã€œé‡å¿ƒï¼‰ï¼šl [m]
- é‡åŠ›åŠ é€Ÿåº¦ï¼šg [m/s^2]
- å°è»Šä½ç½®ï¼šx [m]
- æŒ¯å­è§’åº¦ï¼ˆç›´ç«‹ã‚’0ï¼‰ï¼šÎ¸ [rad]
- å…¥åŠ›ï¼ˆæ°´å¹³åŠ›ï¼‰ï¼šu = F [N]

çŠ¶æ…‹å¤‰æ•°ï¼š

$$
\mathbf{x}=
\begin{bmatrix}
\theta \\
\dot{\theta} \\
x \\
\dot{x}
\end{bmatrix},
\qquad
u = F
$$

---

## 2. éç·šå½¢é‹å‹•æ–¹ç¨‹å¼

$$
(M+m)\ddot{x} + m l \ddot{\theta}\cos\theta - m l \dot{\theta}^2 \sin\theta = u
$$

$$
l\ddot{\theta} + \ddot{x}\cos\theta - g\sin\theta = 0
$$

---

## 3. æ˜ç¤ºå½¢ï¼ˆåŠ é€Ÿåº¦ï¼‰

åˆ†æ¯ã‚’

$$
D(\theta)= (M+m) - m\cos^2\theta
$$

ã¨å®šç¾©ã™ã‚‹ã¨ï¼Œ

$$
\ddot{x} =
\frac{
u + m l \dot{\theta}^2\sin\theta - m g \sin\theta\cos\theta
}{
D(\theta)
}
$$

$$
\ddot{\theta} =
\frac{
u\cos\theta - m l \dot{\theta}^2\sin\theta\cos\theta + (M+m)g\sin\theta
}{
l\,D(\theta)
}
$$

---

## 4. ç·šå½¢åŒ–ï¼ˆç›´ç«‹å¹³è¡¡ç‚¹ï¼‰

è¿‘ä¼¼æ¡ä»¶ï¼š

$$
\theta \approx 0,\quad
\dot{\theta}\approx 0,\quad
x\approx 0,\quad
\dot{x}\approx 0
$$

$$
\sin\theta \approx \theta,\quad
\cos\theta \approx 1
$$

$$
D(0)= (M+m) - m = M
$$

ç·šå½¢åŒ–çµæœï¼š

$$
\ddot{x} \approx \frac{1}{M}u - \frac{m g}{M}\theta
$$

$$
\ddot{\theta} \approx \frac{(M+m)g}{l M}\theta - \frac{1}{lM}u
$$

---

## 5. çŠ¶æ…‹ç©ºé–“è¡¨ç¾

$$
\dot{\mathbf{x}} = A\mathbf{x} + B u
$$

$$
A=
\begin{bmatrix}
0 & 1 & 0 & 0 \\
\frac{(M+m)g}{lM} & 0 & 0 & 0 \\
0 & 0 & 0 & 1 \\
-\frac{mg}{M} & 0 & 0 & 0
\end{bmatrix},
\quad
B=
\begin{bmatrix}
0 \\
-\frac{1}{lM} \\
0 \\
\frac{1}{M}
\end{bmatrix}
$$

---

## 6. å‡ºåŠ›ä¾‹

$$
\mathbf{y}=
\begin{bmatrix}
\theta \\
x
\end{bmatrix}
$$

$$
C=
\begin{bmatrix}
1&0&0&0\\
0&0&1&0
\end{bmatrix},
\quad
D=
\begin{bmatrix}
0\\
0
\end{bmatrix}
$$

---
